The proof of makeSet is done.

sample_mark/verif_unionfind_arr.v
@@ -1,5 +1,6 @@
 Require Import Coq.omega.Omega.
 Require Import VST.floyd.proofauto.
+Require Import RamifyCoq.lib.List_ext.
 Require Import RamifyCoq.sample_mark.env_unionfind_arr.
 Require Import RamifyCoq.graph.graph_model.
 Require Import RamifyCoq.graph.path_lemmas.
@@ -94,21 +95,121 @@ Proof.
     + unfold at_offset. rewrite data_at_rec_eq. simpl. unfold unfold_reptype. simpl. rewrite array_pred_len_0; auto.
 Qed.
 
+Fixpoint prog_list_helper (i: nat) (n: nat) : list (val * val) :=
+  match n with
+  | O => nil
+  | S n' => if (le_dec i n') then (Vundef, Vundef) :: prog_list_helper i n'
+            else (Vint (Int.repr (Z.of_nat (n'))), Vint (Int.repr 0)) :: prog_list_helper i n'
+  end.
+
+Definition progressive_list (i: nat) (n: nat) := rev (prog_list_helper i n).
+
+Lemma progressive_list_repeat: forall n, list_repeat n (Vundef, Vundef) = progressive_list O n.
+Proof.
+  induction n; unfold progressive_list; simpl; auto. unfold progressive_list in IHn. rewrite <- IHn.
+  change ((Vundef, Vundef) :: list_repeat n (Vundef, Vundef)) with (((Vundef, Vundef) :: nil) ++ list_repeat n (Vundef, Vundef)).
+  change ((Vundef, Vundef) :: nil) with (list_repeat 1 (Vundef, Vundef)). rewrite !list_repeat_app. rewrite Nat.add_comm. auto.
+Qed.
+
+Lemma progressive_list_length: forall i n, length (progressive_list i n) = n.
+Proof. intros. unfold progressive_list. rewrite rev_length. induction n; simpl; auto. destruct (le_dec i n); simpl; rewrite IHn; auto. Qed.
+
+Definition progressive_array sh i V rt := data_at sh (tarray vertex_type V) (progressive_list (Z.to_nat i) (Z.to_nat V)) (pointer_val_val rt).
+
+Lemma upd_Znth_twice: forall {A: Type} i (l: list A) v1 v2, 0 <= i < Zlength l -> upd_Znth i (upd_Znth i l v1) v2 = upd_Znth i l v2.
+Proof.
+  intros. unfold upd_Znth. f_equal; [|f_equal].
+  - rewrite sublist0_app1.
+    + rewrite sublist_same; auto. rewrite Zlength_sublist; omega.
+    + rewrite Zlength_sublist; omega.
+  - assert (Zlength (sublist 0 i l) = i) by (rewrite Zlength_sublist; omega). rewrite sublist_app2; rewrite H0. 2: omega.
+    assert (i + 1 - i = 1) by omega. rewrite H1. clear H1. rewrite Zlength_app. rewrite H0. rewrite Zlength_cons. unfold Z.succ.
+    rewrite Zlength_sublist; [|omega..]. assert (i + (Zlength l - (i + 1) + 1) - i = Zlength l - i) by omega. rewrite H1; clear H1.
+    rewrite sublist_1_cons. rewrite sublist_same; [auto | omega |]. rewrite Zlength_sublist; omega.
+Qed.
+
+Lemma prog_list_helper_gt: forall i j n, (i >= n)%nat -> (j >= n)%nat -> prog_list_helper i n = prog_list_helper j n.
+Proof. intros. revert i j H H0. induction n; intros; simpl; auto. destruct (le_dec i n), (le_dec j n); [exfalso; omega ..|]. f_equal. apply IHn; omega. Qed.
+
+Lemma upd_Znth_progressive_list: forall i V,
+    0 <= i < Z.of_nat V -> upd_Znth i (progressive_list (Z.to_nat i) V) (Vint (Int.repr i), Vint (Int.repr 0)) = progressive_list (Z.to_nat (i + 1)) V.
+Proof.
+  intros. induction V. 1: exfalso; simpl in H; intuition. rewrite Nat2Z.inj_succ in H. unfold Z.succ in H. unfold progressive_list. simpl. destruct (le_dec (Z.to_nat i) V).
+  - destruct (le_dec (Z.to_nat (i + 1)) V).
+    + simpl. assert (0 <= i < Z.of_nat V) by (apply inj_le in l0; rewrite Z2Nat.id in l0; omega). unfold progressive_list in IHV. rewrite <- IHV; auto.
+      rewrite upd_Znth_app1; auto. change (rev (prog_list_helper (Z.to_nat i) V)) with (progressive_list (Z.to_nat i) V).
+      rewrite Zlength_correct, progressive_list_length. auto.
+    + assert (Z.to_nat (i + 1) > V)%nat by omega. apply inj_gt in H0. rewrite Z2Nat.id in H0. 2: omega. assert (i = Z.of_nat V) by omega. subst i.
+      clear IHV l n H0 H. rewrite Nat2Z.id. simpl. rewrite upd_Znth_char.
+      * f_equal. change 1 with (Z.of_nat 1). rewrite <- Nat2Z.inj_add, Nat2Z.id. f_equal. apply prog_list_helper_gt; omega.
+      * change (rev (prog_list_helper V V)) with (progressive_list V V). rewrite Zlength_correct, progressive_list_length. auto.
+  - exfalso. assert (Z.to_nat i > V)%nat by omega. apply inj_gt in H0. rewrite Z2Nat.id in H0; omega.
+Qed.
+
+Fixpoint nat_inc_list (n: nat) : list Z :=
+  match n with
+  | O => nil
+  | S n' => nat_inc_list n' ++ (Z.of_nat n' :: nil)
+  end.
+
+Lemma nat_inc_list_in_iff: forall n v, In v (nat_inc_list n) <-> 0 <= v < Z.of_nat n.
+Proof.
+  induction n; intros; [simpl; intuition|]. rewrite Nat2Z.inj_succ. unfold Z.succ. simpl. rewrite in_app.
+  assert (0 <= v < Z.of_nat n + 1 <-> 0 <= v < Z.of_nat n \/ v = Z.of_nat n) by omega. rewrite H. clear H. rewrite IHn. simpl. intuition.
+Qed.
+
+Lemma nat_inc_list_NoDup: forall n, NoDup (nat_inc_list n).
+Proof.
+  induction n; simpl; [constructor|]. apply NoDup_app_inv; auto.
+  - constructor; auto. constructor.
+  - intros. rewrite nat_inc_list_in_iff in H. simpl. omega.
+Qed.
+
+Lemma nat_inc_list_length: forall n, length (nat_inc_list n) = n. Proof. induction n; simpl; auto. rewrite app_length. simpl. rewrite IHn. intuition. Qed.
+
+Lemma progressive_nat_inc_list: forall n i, (i >= n)%nat -> map (fun x : Z => (Vint (Int.repr x), Vint (Int.repr 0))) (nat_inc_list n) = progressive_list i n.
+Proof.
+  induction n; intros; unfold progressive_list in *; simpl; auto. destruct (le_dec i n). 1: exfalso; omega. rewrite map_app. simpl. rewrite <- IHn; intuition.
+Qed.
+
 Lemma body_makeSet: semax_body Vprog Gprog f_makeSet makeSet_spec.
 Proof.
   start_function. forward_call (sh, Z.mul V 8).
   - split. 1: omega. assert (Z.mul 8 (Int.max_signed /8) <= Int.max_signed) by (apply Z_mult_div_ge; intuition).
     apply Z.le_trans with Int.max_signed. 1: omega. rewrite Z.lt_eq_cases; left; apply Int.max_signed_unsigned.
-  - Intro rt.
+  - Intro rt. Intros.
+    assert (memory_block sh (V * 8) (pointer_val_val rt) = data_at_ sh (tarray vertex_type V) (pointer_val_val rt)). {
+      assert (memory_block sh (V * 8) (pointer_val_val rt) = memory_block sh (sizeof (tarray vertex_type V)) (pointer_val_val rt)). {
+        simpl sizeof. rewrite Zmax0r. 2: intuition. assert (V * 8 = 8 * V)%Z by omega. rewrite H1. auto.
+      } rewrite <- memory_block_data_at_; auto. apply malloc_compatible_field_compatible; auto.
+      - unfold malloc_compatible in *. destruct (pointer_val_val rt); auto. destruct H0. split; auto. simpl sizeof. rewrite Zmax0r; intuition.
+      - unfold legal_alignas_type, nested_pred. simpl. compute. destruct V; auto. exfalso. destruct H. pose proof (Zlt_neg_0 p). intuition.
+      - exists 2. compute. auto.
+    } rewrite H1. clear H1.
+    assert (data_at_ sh (tarray vertex_type V) (pointer_val_val rt) = data_at sh (tarray vertex_type V) (progressive_list O (Z.to_nat V)) (pointer_val_val rt)). {
+      unfold data_at_, field_at_, data_at. assert (default_val (nested_field_type (tarray vertex_type V) []) = list_repeat (Z.to_nat V) (Vundef, Vundef)) by reflexivity.
+      rewrite H1. rewrite progressive_list_repeat. auto.
+    } rewrite H1. clear H1.
     forward_for_simple_bound V 
       (EX i: Z,
-       PROP (forall m : Z, 0 <= m < i -> vvalid (makeSet_discrete_Graph (Z.to_nat i)) m)
-       LOCAL (temp _subsets (pointer_val_val rt))
-       SEP (whole_graph sh (makeSet_discrete_Graph (Z.to_nat i)) rt; memory_block sh ((V - i) * 8) (pointer_val_val rt))).
+       PROP ()
+       LOCAL (temp _subsets (pointer_val_val rt); temp _V (Vint (Int.repr V)))
+       SEP (progressive_array sh i V rt)); unfold progressive_array.
     + destruct H. apply Z.le_trans with (Int.max_signed / 8); auto. rewrite Z.lt_eq_cases. left. apply Z_div_lt; intuition.
-    + simpl Z.to_nat. Intros. rewrite (whole_graph_empty _ _ (V * 8)); auto. 2: omega. assert (V - 0 = V) by omega. rewrite H1. clear H1. entailer.
-    + Intros. eapply semax_seq'. admit.
-    + assert (((V - V) * 8)%Z = 0) by omega. rewrite H0; clear H0. rewrite memory_block_zero. forward. apply (exp_right (makeSet_discrete_Graph (Z.to_nat V))).
-      entailer. apply (exp_right rt). entailer.
-      
-Abort.
+    + entailer.
+    + Opaque Znth. forward. remember (Znth i (progressive_list (Z.to_nat i) (Z.to_nat V)) (Vundef, Vundef)) as lll. destruct lll. forward.
+      assert (0 <= i < Zlength (progressive_list (Z.to_nat i) (Z.to_nat V))) by (split; [|rewrite Zlength_correct, progressive_list_length, Z2Nat.id]; omega).
+      rewrite upd_Znth_same, upd_Znth_twice; [|auto ..]. unfold progressive_array, data_at.
+      rewrite upd_Znth_progressive_list. 2: rewrite Z2Nat.id; omega. entailer.
+    + forward. apply (exp_right (makeSet_discrete_Graph (Z.to_nat V))). entailer. apply (exp_right rt). entailer. apply andp_right.
+      * apply prop_right. intros. simpl. rewrite makeSet_vvalid. rewrite Z2Nat.id; omega.
+      * unfold whole_graph, full_graph_at. simpl. unfold graph_vcell_at. apply (exp_right (nat_inc_list (Z.to_nat V))).
+        apply andp_right; [apply andp_right; apply prop_right |]; intros.
+        -- rewrite makeSet_vvalid. rewrite nat_inc_list_in_iff. intuition.
+        -- apply nat_inc_list_NoDup.
+        -- simpl. unfold vcell_array_at, SAG_VST. rewrite map_length, nat_inc_list_length. rewrite Z2Nat.id. 2: intuition.
+           assert (map (fun x : Z => vgamma (makeSet_discrete_LabeledGraph (Z.to_nat V)) x) (nat_inc_list (Z.to_nat V)) =
+                   map (fun x => (0%nat, x)) (nat_inc_list (Z.to_nat V))). {
+             apply list_map_exten. intros. unfold vgamma. simpl. rewrite makeSet_dst. simpl. auto.
+           } rewrite H6. clear H6. rewrite list_map_compose. unfold vgamma2cdata. simpl. rewrite <- progressive_nat_inc_list; intuition. 
+Qed.
